\documentclass[12pt]{article}
\usepackage{amsmath, amssymb, amsthm}
\usepackage{geometry}
% \geometry{letterpaper, margin=1in}

\newtheorem{proposition}{Proposition}
\newcommand{\ddx}{\frac{d}{dx}}

\begin{document}

\title{Sum Rule}
\author{Hanson Jiang}
\maketitle

\begin{proposition}
  $\forall f, g,$ both differentiable at $c$,
  $\ddx (f(x)+g(x)) = \ddx f(x) + \ddx g(x)$.

\end{proposition}

\begin{proof}
  \begin{align*}
    \ddx f(x) + \ddx g(x)
    &=\lim_{x\rightarrow c} \frac{f(x)-f(c)}{x-c}
    +\lim_{x\rightarrow c} \frac{g(x)-g(c)}{x-c} \\
    &= \lim_{x\rightarrow c} \frac{f(x)-f(c)}{x-c} + \frac{g(x)-g(c)}{x-c} \\
    &= \lim_{x\rightarrow c} \frac{f(x)-f(c) + g(x)-g (c)}{x-c} \\
    &= \lim_{x\rightarrow c} \frac{(f(x)+g(x)) - (f(c)+g (c))}{x-c} \\
    &= \ddx (f(x)+g(x))
  \end{align*}
\end{proof}

\end{document}